src/ItreeExtra/Dijkstra/DelaySpecMonad.v
@@ -1,0 +1,280 @@
+From Coq Require Import
+     Morphisms.
+
+From ExtLib Require Import
+     Structures.Monad.
+
+From ITree Require Import
+     ITree
+     ITreeFacts
+     Props.Infinite.
+
+From ITree.Extra Require Import
+     Dijkstra.DijkstraMonad
+     Dijkstra.PureITreeBasics
+     Dijkstra.IterRel.
+
+From Paco Require Import paco.
+
+Import Monads.
+Import MonadNotation.
+
+#[local] Open Scope monad_scope.
+
+Set Implicit Arguments.
+
+(** Contains the DelaySpec monad, the specification monad for partial computations with no uninterpretted effects. Also contains an effect observation from the Delay monad into  the DelaySpec monad along with a proof that it is a monad morphism. Also contains a loop invariant principle for iter over Delay*)
+
+Ltac clear_ret_eutt_spin :=
+  match goal with | H : ret ?a ≈ ITree.spin  |- _ => simpl in H; exfalso; eapply not_ret_eutt_spin; eauto
+             | H : Ret ?a ≈ ITree.spin  |- _ => exfalso; eapply not_ret_eutt_spin; eauto
+             | H : ITree.spin ≈ ret ?a  |- _ => exfalso; symmetry in H; eapply not_ret_eutt_spin; eauto
+             | H : any_infinite (ret _ ) |- _ => pinversion H
+  end.
+
+Ltac invert_evidence :=
+  intros; repeat match goal with
+                 | H : _ /\ _ |- _ => destruct H
+                 | H : _ \/ _ |- _ => destruct H
+                 | H : exists a : ?A, _ |- _ => destruct H as [?a ?H]
+                 | x : ?A + ?B |- _ => destruct x as [?a | ?b]
+                 | H : upaco1 _ _ _ |- _ => pclearbot
+                 end.
+
+Ltac invert_ret := simpl in *; match goal with | H : Ret ?a ≈ Ret ?b |- _ =>
+                                                 apply eutt_inv_Ret in H; try discriminate; try (injection H as H);
+                                                 subst end.
+
+
+Ltac basic_solve := invert_evidence; try clear_ret_eutt_spin; try invert_ret.
+
+Ltac dest_dep f a := destruct (f a) as [?fa ?Hfa] eqn : ?Heq; simpl in *.
+
+Declare Scope delayspec_scope.
+Delimit Scope delayspec_scope with delayspec.
+
+#[local] Open Scope delayspec_scope.
+
+Notation "a ∈ b" := (proj1_sig (A := _ -> Prop) b a) (at level 70) : delayspec_scope.
+Notation "a ∋ b" := (proj1_sig (A := _ -> Prop) a b) (at level 70, only parsing) : delayspec_scope.
+
+Definition Delay (A : Type) := itree void1 A.
+
+#[global] Instance EqMDelay : Eq1 Delay := @ITreeMonad.Eq1_ITree void1.
+#[global] Instance MonadDelay : Monad Delay := @Monad_itree void1.
+#[global] Instance MonadIterDelay : MonadIter Delay := fun R I f a => ITree.iter f a.
+
+Definition DelaySpecInput (A : Type) : Type := {p : Delay A -> Prop | resp_eutt p}.
+
+Definition DelayIn {A : Type} (t : Delay A) (p : DelaySpecInput A) : Prop := proj1_sig p t.
+
+Definition DelaySpec (A : Type) : Type :=
+  { w : DelaySpecInput A -> Prop
+  | forall (p p' : DelaySpecInput A), (forall t, t ∈ p -> t ∈ p') -> w p -> w p'}.
+
+#[program] Definition ret_del (A : Type) (a : A) : DelaySpec A := fun p => p (Ret a).
+
+#[program] Definition _bind_del (A B : Type) (w : DelaySpec A) (f : A -> DelaySpec B)
+  : DelaySpecInput B -> Prop :=
+  fun p => w ∋ (fun t => (exists a, Ret a ≈ t /\ p ∈ f a) \/ (any_infinite t /\ p ITree.spin)).
+Next Obligation.
+  intros t1 t2 Heutt. split; intros; basic_solve.
+  - left. exists a. split; auto. rewrite H. auto.
+  - right. rewrite <- Heutt. auto.
+  - left. exists a. rewrite Heutt. auto.
+  - right. rewrite Heutt. auto.
+Qed.
+
+#[program] Definition bind_del (A B : Type) (w : DelaySpec A) (f : A -> DelaySpec B) : DelaySpec B :=
+  _bind_del w f.
+Next Obligation.
+  red. red in H0. destruct w as [w Hw]. simpl in *. eapply Hw; try apply H0.
+  simpl. intros. basic_solve.
+  - left. exists a. split; auto. dest_dep f a. eapply Hfa; eauto.
+  - right. split; auto.
+Qed.
+
+#[global] Instance DelaySpecEq : Eq1 DelaySpec :=
+  fun _ w1 w2 => forall p, p ∈ w1 <-> p ∈ w2.
+
+#[global] Instance DelaySpecEqEquiv {A : Type} : Equivalence (A := DelaySpec A) eq1.
+Proof.
+  constructor; repeat intro; try tauto.
+  - repeat red in H. specialize (H p). tauto.
+  - repeat red in H, H0. specialize (H p). specialize (H0 p). tauto.
+Qed.
+
+#[global] Instance DelaySpecMonad : Monad DelaySpec :=
+  {
+    ret := ret_del;
+    bind := bind_del
+  }.
+
+#[program, global]
+Instance DelaySpecMonadLaws : MonadLawsE DelaySpec.
+Next Obligation.
+  repeat red. cbn. split; intros; basic_solve; auto.
+  - pinversion H.
+  - left. exists x. split; auto; reflexivity.
+Qed.
+Next Obligation.
+  rename x into w.
+  repeat red. cbn. split; intros.
+  - red in H. simpl in H. destruct w as [w Hw]. simpl in *. eapply Hw; try apply H.
+    intros. simpl in *. destruct p as [p Hp]. simpl in *. basic_solve.
+    + eapply Hp; eauto. symmetry. auto.
+    + apply div_spin_eutt in H0. eapply Hp; eauto.
+  - red. destruct w as [w Hw]. simpl in *. eapply Hw; try apply H. intros.
+    destruct p as [p Hp]. simpl in *.
+    destruct (eutt_reta_or_div t); basic_solve.
+    + left. exists a. split; auto. eapply Hp; eauto.
+    + right. split; auto. eapply Hp; try apply H0. symmetry. apply div_spin_eutt. auto.
+Qed.
+Next Obligation.
+  rename x into w.
+  repeat red. cbn. split; intros.
+  - red. red in H. destruct w as [w Hw]. simpl in *. destruct p as [p Hp]. simpl in *.
+    eapply Hw; try apply H. intros. simpl in *. clear H. basic_solve.
+    + left. exists a. auto.
+    + right. auto.
+  - red. red in H. destruct w as [w Hw]. simpl in *. destruct p as [p Hp]. simpl in *.
+    eapply Hw; try apply H. simpl in *. intros. basic_solve.
+    + left. exists a. auto.
+    + right. split; auto. right. split; try auto using spin_infinite.
+Qed.
+Next Obligation.
+  intros w1 w2 Hw k1 k2 Hk. unfold pointwise_relation in Hk.
+  repeat red. unfold bind_del, _bind_del; split; intros; destruct w1 as [w1 Hw1];
+                destruct w2 as [w2 Hw2]; do 2 red in Hw;
+                  simpl in *.
+  - rewrite <- Hw. eapply Hw1; try apply H; simpl in *. intros.
+    destruct H0 as [ [a [Ht Ha] ] | [Hdiv Hspin] ]; auto.
+    left. exists a. split; auto.
+    specialize (Hk a). destruct (k1 a) as [k1a Hk1a];
+                         destruct (k2 a) as [k2a Hk2a];
+                         do 2 red in Hk; simpl in *.
+    apply Hk. auto.
+  - rewrite Hw. eapply Hw2; try apply H; simpl in *. intros.
+    destruct H0 as [ [a [Ht Ha] ] | [Hdiv Hspin] ]; auto.
+    left. exists a. split; auto.
+    specialize (Hk a). destruct (k1 a) as [k1a Hk1a];
+                         destruct (k2 a) as [k2a Hk2a];
+                         do 2 red in Hk; simpl in *.
+    apply Hk. auto.
+Qed.
+
+#[global] Instance DelaySpecOrderM : OrderM DelaySpec :=
+  fun _ w1 w2 => forall p, p ∈ w2 -> p ∈ w1.
+
+#[global] Instance DelaySpecOrder : OrderedMonad DelaySpec.
+Proof.
+  constructor.
+  - intros. repeat red. intros. destruct w. auto.
+  - intros. destruct w1. destruct w2. destruct w3. intro. simpl in *.
+    specialize (H p2). specialize (H0 p2). simpl in *. intros. auto.
+  - red. intros. repeat red. cbn. destruct w1 as [w1 Hw1]. destruct w2 as [w2 Hw2].
+    intros. simpl in *. apply H. simpl in *. eapply Hw2; try apply H1. simpl in *. intros.
+    basic_solve.
+    + left. exists a. split; auto. apply H0. auto.
+    + right. auto.
+Qed.
+
+#[program] Definition obs_del (A : Type) (t : Delay A) : DelaySpec A := fun p => t ∈ p.
+
+#[global] Instance DelaySpecObs : EffectObs Delay DelaySpec := obs_del.
+
+#[global] Instance DelaySpecMonadMorph : MonadMorphism Delay DelaySpec DelaySpecObs.
+Proof.
+  constructor.
+  - repeat red. cbn. tauto.
+  - repeat red. cbn. split; intros; basic_solve.
+    + destruct (eutt_reta_or_div m); basic_solve.
+      * left. exists a. split; auto. destruct p as [p Hp]. simpl in *. eapply Hp; try apply H.
+        rewrite <- H0. setoid_rewrite bind_ret_l. reflexivity.
+      * right. split; auto. apply div_spin_eutt in H0. destruct p as [p Hp]. eapply Hp; try apply H.
+        rewrite H0. apply spin_bind.
+    + destruct p as [p Hp]. simpl in *. eapply Hp; try apply H0. rewrite <- H. setoid_rewrite bind_ret_l. reflexivity.
+    + apply div_spin_eutt in H. destruct p as [p Hp]. simpl in *. eapply Hp; try apply H0. rewrite H.
+      symmetry. apply spin_bind.
+Qed.
+
+Definition iter_arrow_rel {A B : Type} (g : A -> Delay (A + B) ) (a1 a2 : A) : Prop :=
+  g a1 ≈ ret (inl a2).
+
+Notation "x =[ g ]=> y" := (iter_arrow_rel g x y) (at level 70) : delayspec_scope.
+
+Lemma iter_inl_spin : forall (A B : Type) (g : A -> Delay (A + B) ) (a : A),
+    not_wf_from (iter_arrow_rel g) a -> ITree.iter g a ≈ ITree.spin.
+Proof.
+  intros A B g. einit. ecofix CIH. intros. pinversion H0; try apply not_wf_F_mono'.
+  setoid_rewrite unfold_iter_ktree. unfold iter_arrow_rel in Hrel. apply eutt_ret_euttge in Hrel.
+  rewrite Hrel. rewrite bind_ret_l. rewrite unfold_spin. etau.
+Qed.
+
+(*eventually might want more general reasoning principle, like weaken the second precondition to only apply
+  to a' reachable from a under g*)
+Lemma iter_wf_converge : forall (A B : Type) (g : A -> Delay (A + B) ) (a : A),
+    wf_from (iter_arrow_rel g) a ->
+    (forall a, exists (ab : A + B), g a ≈ Ret ab) ->
+    exists b : B, ITree.iter g a ≈ Ret b.
+Proof.
+  intros A B g a Hwf Hconv.
+  induction Hwf.
+  - specialize (Hconv a). destruct Hconv as [ [a' | b] Hret ].
+    + exfalso. apply (H a'). auto.
+    + exists b. rewrite unfold_iter. rewrite Hret. rewrite bind_ret_l.
+      reflexivity.
+  - specialize (Hconv a). destruct Hconv as [ [a' | b] Hret ].
+    + apply H0 in Hret as Hret'. destruct Hret' as [b Hret']. exists b.
+      rewrite unfold_iter. rewrite Hret. rewrite bind_ret_l. rewrite tau_eutt. auto.
+    + exists b. rewrite unfold_iter. rewrite Hret. rewrite bind_ret_l.
+      reflexivity.
+Qed.
+
+
+Definition loop_invar_imp {A B : Type} (q : Delay (A + B) -> Prop) (p : Delay B -> Prop) :Prop :=
+  forall t, q (t >>= fun b => ret (inr b) ) -> p t.
+
+Definition iter_lift {A B : Type} (g : A -> Delay (A + B)) : (A + B) -> Delay (A + B) :=
+  fun x => match x with
+             | inl a => g a
+             | inr b => ret (inr b) end.
+
+Notation "q -+> p" := (loop_invar_imp q p) (at level 80) : delayspec_scope.
+
+Lemma loop_invar : forall (A B : Type) (g : A -> Delay (A + B) ) (a : A)
+                          (p : Delay B -> Prop) (Hp : resp_eutt p)
+                          (q : Delay (A + B) -> Prop) (Hq : resp_eutt q),
+    (q -+> p) -> (q (g a)) ->
+    (forall t, q t -> q (bind t (iter_lift g))) ->
+    (p \1/ any_infinite) (ITree.iter g a).
+Proof.
+  intros. unfold loop_invar_imp in *.
+  set (iter_arrow_rel g) as rg.
+  destruct (classic_wf rg a).
+  - left. induction H2.
+    + unfold rg, iter_arrow_rel in H2. destruct (eutt_reta_or_div (g a)); basic_solve.
+      * symmetry in H3. apply H2 in H3. contradiction.
+      * apply H. cbn. eapply Hq; try apply H0.
+        setoid_rewrite unfold_iter_ktree. rewrite <- H3.
+        repeat setoid_rewrite bind_ret_l. reflexivity.
+      * apply div_spin_eutt in H3. apply H. cbn.
+        eapply Hq; try apply H0. rewrite H3.
+        setoid_rewrite unfold_iter. rewrite H3.
+        symmetry. setoid_rewrite <- spin_bind. apply spin_bind.
+    + unfold rg in *.
+      destruct (eutt_reta_or_div (g a)); basic_solve.
+      * cbn in H4. rewrite unfold_iter, <- H4, bind_ret_l, tau_eutt.
+        apply H3.
+        -- red. symmetry; assumption.
+        -- unfold iter_lift in H1. specialize (H1 (g a) H0).
+           eapply Hq; try apply H1. cbn. rewrite <- H4. setoid_rewrite bind_ret_l.
+           reflexivity.
+      * cbn in H4. rewrite unfold_iter, <- H4, bind_ret_l.
+        apply H. cbn. rewrite bind_ret_l. eapply Hq; eauto.
+      * apply div_spin_eutt in H4. apply H. cbn.
+        eapply Hq; try apply H0. rewrite H4.
+        setoid_rewrite unfold_iter. rewrite H4. repeat setoid_rewrite <- spin_bind.
+        reflexivity.
+  - apply iter_inl_spin in H2. right. rewrite H2. apply spin_infinite.
+Qed.
