src/ItreeExtra/Dijkstra/PureITreeDijkstra.v
@@ -1,0 +1,651 @@
+From ExtLib Require Import
+     Structures.Monad.
+
+From Paco Require Import paco.
+
+From ITree Require Import
+     Indexed.Sum
+     ITree
+     ITreeFacts
+     Props.Infinite.
+
+From ITree.Extra Require Import
+     Dijkstra.DijkstraMonad
+     Dijkstra.PureITreeBasics.
+
+Import Monads.
+Import MonadNotation.
+#[local] Open Scope monad_scope.
+
+Section PureITree.
+
+  Definition PureITree A := itree void1 A.
+
+  (*Morally, this is the type of pure itree specifcations. A sigma of this with a monotonicity requiremnet is used
+    in order to proved the ordered monad law*)
+  Definition _PureITreeSpec A := forall (p : itree void1 A -> Prop), resp_eutt p -> Prop.
+
+
+
+  (*Monotonicity condition for specs on pure itrees*)
+  Definition monotonici A (w : _PureITreeSpec A) :=
+    forall (p p' : itree void1 A -> Prop) (Hp : resp_eutt p) (Hp' : resp_eutt p'),
+                                          (forall i', p i' -> p' i') -> w p Hp -> w p' Hp'.
+
+  (* same as monot  *)
+  Definition dmonot A (w : _PureITreeSpec A) :=
+    forall (p p' : itree void1 A -> Prop) Hp Hp', (forall t, p t <-> p' t) -> (w p Hp <-> w p' Hp').
+  (* what if we identify a spec with the intersection of all of the preds it accepts*)
+  Lemma monot_imp_dmonot : forall A (w : _PureITreeSpec A), monotonici A w -> dmonot A w.
+  Proof.
+    unfold monotonici, dmonot. intros. split.
+    - apply H; auto. intros. apply H0. auto.
+    - apply H; auto. intros. apply H0. auto.
+  Qed.
+
+  (* does not hold for many basic specs  *)
+  Definition amonot A (w : _PureITreeSpec A) :=
+    forall (p p' : itree void1 A -> Prop) Hp Hp', (forall t, p t -> p' t) -> w p' Hp' -> w p Hp.
+
+  (*Sigm*)
+  Definition PureITreeSpec A := {w : _PureITreeSpec A | monotonici A w}.
+
+  (*The set of predicates that accept divergent trees*)
+  Definition _div_spec A : _PureITreeSpec A := fun p _ => p ITree.spin.
+
+  Lemma div_spec_monot : forall A, monotonici A (_div_spec A).
+    Proof.
+      unfold monotonici, _div_spec. auto.
+    Qed.
+
+  Lemma div_spec_amonot : forall A , amonot A (_div_spec A).
+  Proof.
+    unfold amonot, _div_spec. intros. auto.
+  Abort.
+  Definition div_spec A := exist _ (_div_spec A) (div_spec_monot A).
+
+  (*Morally, this is the return function. This is paired with a proof that all such specs are monotonic*)
+  Definition _retpi A (a : A) : _PureITreeSpec A := fun p _ => p (ret a).
+
+  Lemma retpi_monot : forall A (a : A), monotonici A (_retpi A a).
+  Proof.
+    unfold monotonici. intuition. unfold _retpi in *. auto.
+  Qed.
+
+  Lemma retpi_amonot : forall A (a : A), amonot A ( _retpi A a ).
+  Proof.
+    unfold amonot, _retpi. intros.
+    Abort.
+
+  (*Proof that the predicate used in the bind function respects eutt*)
+  Lemma bind_pred_resp_eutt : forall A B (f : A -> _PureITreeSpec B)
+                                     (p : itree void1 B -> Prop) (Hp : resp_eutt p),
+      resp_eutt (fun (t : itree void1 A) => (exists a, ret a ≈ t /\ f a p Hp) \/
+                                            (any_infinite t /\ p ITree.spin)).
+  Proof.
+    intros. intros t1 t2 Heutt. setoid_rewrite Heutt. reflexivity.
+  Qed.
+
+  (*the bind function for the PureITreeSpec monad
+    intuitively, you have two choices, prove the tree evaluates to a and prove f a p,
+    or prove t is infinite and prove that the infinite predicate is in w*)
+  Definition _bindpi A B (w : _PureITreeSpec A) (f : A -> _PureITreeSpec B) : _PureITreeSpec B :=
+    fun (p : itree void1 B -> Prop) (Hp : resp_eutt p) =>
+      w (fun (t : itree void1 A) => (exists a, ret a ≈ t /\ f a p Hp) \/
+                                    (any_infinite t /\ p ITree.spin ))
+        (bind_pred_resp_eutt A B f p Hp).
+
+  Lemma bindpi_monot : forall A B (w : _PureITreeSpec A) (f : A -> _PureITreeSpec B),
+      monotonici A w -> (forall a, monotonici B (f a)) -> monotonici B (_bindpi A B w f).
+  Proof.
+    unfold monotonici. intros. unfold _bindpi in *.
+    set (fun (t : itree void1 A) p0 Hp0 =>
+      (exists a, ret a ≈ t /\ f a p0 Hp0) \/ (any_infinite t /\ p ITree.spin))  as fp.
+    enough (forall t, fp t p Hp -> fp t p' Hp').
+    - eapply H with (p := fun t => fp t p Hp).
+      + intros.  apply H3 in H4.
+        unfold fp in H4. destruct H4; auto.
+        destruct H4. right. auto.
+      + apply H2.
+    - unfold fp. intros. destruct H3; auto. left.
+      intros. destruct H3 as [a [Hvala Hfa] ].
+      exists a. split; auto.
+      eapply H0; [ eauto | ].
+      revert Hfa; apply H0; auto.
+  Qed.
+
+  (*Definition of ret accounting for the proof of monotonicity*)
+  Definition retpi A (a : A) : PureITreeSpec A :=
+    exist _ (_retpi A a) (retpi_monot A a).
+
+  (*Definition of bind accounting for the proof of monotonicity*)
+  Definition bindpi A B (w : PureITreeSpec A) (f : A -> PureITreeSpec B) :=
+    let '(exist _ w' Hw') := w in
+    let f' := fun a => proj1_sig (f a) in
+    let Hf' := fun a => proj2_sig (f a) in
+    exist _ (_bindpi A B w' f') (bindpi_monot A B w' f' Hw' Hf').
+
+  Lemma inf_tree_pred_resp_eutt : forall A B (p : itree void1 B -> Prop),
+      resp_eutt (fun (t : itree void1 (A+B)) => any_infinite t /\ p ITree.spin).
+  Proof.
+    intros. intros t1 t2 Heutt. rewrite Heutt. reflexivity.
+  Qed.
+
+  Lemma term_b_pred_resp_eutt : forall A B (p : itree void1 B -> Prop),
+      resp_eutt (fun (t : itree void1 (A + B)) => exists b, ret (inr b) ≈ t /\ p (ret b)  ).
+  Proof.
+    intros. intros t1 t2 Heutt. split; intros.
+    - destruct H. exists x. rewrite <- Heutt. auto.
+    - destruct H. exists x. rewrite Heutt. auto.
+  Qed.
+
+  Lemma cont_a_pred_resp_eutt : forall A B
+                                       (F : A -> Prop),
+      resp_eutt (fun (t : itree void1 (A + B)) => exists a' , ret (inl a') ≈ t /\ F a'  ).
+  Proof.
+    intros. intros t1 t2 Heutt. split; intros.
+    - destruct H. exists x. rewrite <- Heutt. auto.
+    - destruct H. exists x. rewrite Heutt. auto.
+  Qed.
+
+  Lemma resp_eutt_or : forall A (p p' : itree void1 A -> Prop),
+      resp_eutt p -> resp_eutt p' -> resp_eutt (fun t => p t \/ p' t).
+  Proof.
+    intros. intros t1 t2 Ht. split; intros.
+    - destruct  H1.
+      + left. eapply H; eauto. symmetry. auto.
+      + right. eapply H0; eauto. symmetry. auto.
+    - destruct H1.
+      + left. eapply H; eauto.
+      + right. eapply H0; eauto.
+  Qed.
+
+  Definition iterF_body' {A B : Type}
+            (p : itree void1 B -> Prop) (Hp : resp_eutt p) (F : A -> Prop) :=
+    fun (t : itree void1 (A + B) ) =>( any_infinite t /\ p ITree.spin) \/
+                                    (exists b, ret (inr b) ≈ t /\ p (ret b)  ) \/
+                                    (exists a', ret (inl a') ≈ t /\ F a').
+
+  Variant iterF_body {A B : Type}
+            (p : itree void1 B -> Prop) (Hp : resp_eutt p) (F : A -> Prop)
+            (t : itree void1 (A + B)) : Prop :=
+    | inf_tau (Ht: any_infinite t) (Hspin : p ITree.spin)
+    | term_b (b : B) (Hretb : ret (inr b) ≈ t ) (Hb : p (ret b))
+    | cont_a (a' : A) (Hreta : ret (inl a') ≈ t) (Hcorec : F a')
+.
+
+ Lemma iterF_body_equiv : forall A B
+            (p : itree void1 B -> Prop) (Hp : resp_eutt p) (F : A -> Prop)
+            (t : itree void1 (A + B)), iterF_body p Hp F t <-> iterF_body p Hp F t.
+   Proof.
+     split; intros; auto.
+   Qed.
+
+Hint Constructors iterF_body : itree.
+
+  Lemma iterF_body'_resp_eutt : forall (A B : Type)
+            (p : itree void1 B -> Prop) (Hp : resp_eutt p) (F : A -> Prop),
+      resp_eutt (iterF_body' p Hp F).
+  Proof.
+    intros. eapply resp_eutt_or; try eapply resp_eutt_or; intros.
+    - apply inf_tree_pred_resp_eutt.
+    - apply term_b_pred_resp_eutt.
+    - apply cont_a_pred_resp_eutt.
+  Qed.
+
+  Lemma iterF_body_resp_eutt : forall (A B : Type)
+            (p : itree void1 B -> Prop) (Hp : resp_eutt p) (F : A -> Prop),
+      resp_eutt (iterF_body p Hp F).
+  Proof.
+    intros. intros t1 t2 Heutt. split; intros; inversion H; subst; auto.
+    - apply inf_tau; auto. rewrite Heutt in Ht. auto.
+    - eapply term_b; eauto. rewrite Hretb. auto.
+    - eapply cont_a; eauto. rewrite Hreta. auto.
+    - apply inf_tau; auto. rewrite Heutt. auto.
+    - eapply term_b; eauto. rewrite Hretb. symmetry. auto.
+    - eapply cont_a; eauto. rewrite Hreta. symmetry. auto.
+  Qed.
+
+  Variant iterF {A B : Type} (body : A -> PureITreeSpec (A + B))
+          (a : A) (p : itree void1 B -> Prop) (Hp : resp_eutt p) (F : A -> Prop) : Prop :=
+    | iterF_con : proj1_sig (body a) (iterF_body p Hp F) (iterF_body_resp_eutt A B p Hp F) -> iterF body a p Hp F.
+
+(*
+  Inductive iter_ind {A B : Type} (f : A -> PureITreeSpec (A + B) ) (a : A) (p : itree void1 B -> Prop)
+           (Hp : resp_eutt _ _ p) : Prop :=
+    | iter_ind_cons (Hiter : iterF f a p Hp (fun a0 => iter_ind f a0 p Hp) ) .
+*)
+(*
+  Lemma
+
+  Inductive iter_ind {A B : Type} (body : A -> _PureITreeSpec (A + B) ) (p : itree void1 B -> Prop)
+            (Hp : resp_eutt _ _ p) : A -> Prop :=
+    | Hiter (a : A) : body a (fun t : itree void1 (A + B) => (any_infinite t /\ p spin)
+                                                   \/ (exists b, t ≈ (ret (inr b) /\ p (ret b) ))
+                                             \/ (exists a', t ≈ (ret (inl a')) /\
+                                         iter_ind body p Hp a') ) .
+*)
+Hint Constructors iterF : itree.
+Lemma iterF_monotone {A B} (body:  (A -> PureITreeSpec (A + B)))
+      (sim sim' : A -> Prop) (a : A)
+      (p : itree void1 B -> Prop) (Hp : resp_eutt p)
+      (IN : iterF body a p Hp sim) (LE : sim <1= sim'):
+  iterF body a p Hp sim'.
+  Proof.
+    induction IN; constructor; auto.
+    destruct (body a) as [fa Hfa] eqn : Heq. simpl in *.
+    refine (Hfa _ _ _ _ _ H). intros. inversion H0; eauto with itree.
+  Qed.
+
+  Definition iter_ {A B} sim (body : A -> PureITreeSpec (A + B)) a p Hp : Prop :=
+    iterF body a p Hp sim.
+  Hint Unfold iter_ : itree.
+
+  Lemma iterF_monotone' {A B} body p Hp : monotone1 (fun sim a => @iter_ A B sim body a p Hp).
+  Proof.
+    do 2 red. intros. eapply iterF_monotone; eauto.
+  Qed.
+
+  Hint Resolve iterF_monotone' : paco.
+
+  Definition _iter {A B} :=
+    fun (f : A -> PureITreeSpec (A + B) ) (a : A) (p : itree void1 B -> Prop) (Hp : resp_eutt p) =>
+      paco1 (fun (F : A -> Prop) a => @iter_ A B F f a p Hp ) bot1 a.
+
+
+
+  Lemma iter_monot : forall A B (f : A -> PureITreeSpec (A + B) ) (a : A),
+                              monotonici B (_iter f a).
+    Proof.
+      unfold monotonici. intros. generalize dependent a.
+      pcofix CIH. pfold. intros. punfold H1.
+      red. red in H1. inversion H1; simpl in *.
+      constructor. destruct (f a) as [fa Hfa] eqn : Heq. simpl in *.
+      refine (Hfa _ _ _ _ _ H0). intros t. intros. inversion H2; subst; eauto with itree.
+      pclearbot. eapply cont_a; eauto with itree.
+    Qed.
+
+  Definition iterp {A B} (body : A -> PureITreeSpec (A + B) ) (init : A) : PureITreeSpec B :=
+    exist _ (_iter body init) (iter_monot A B body init).
+
+(*there may be a way to reason about iteration in spec monads *)
+
+  (*Monad equivalence relation for PureITreeSpec monad *)
+  #[global] Instance PureITreeSpecEq : Eq1 PureITreeSpec :=
+    fun A w1 w2 => forall (p : itree void1 A -> Prop) (Hp : resp_eutt p), proj1_sig w1 p Hp <-> proj1_sig w2 p Hp.
+
+  #[global] Instance PureItreeSpecMonad : Monad PureITreeSpec :=
+    {
+      ret := retpi;
+      bind := bindpi
+    }.
+
+  (*Monad law proofs*)
+  Lemma retpi_bindpi : forall A B (f : A -> PureITreeSpec B) (a : A),
+      (bind (ret a) f ≈ f a)%monad.
+  Proof.
+    intros. split.
+    - cbn. unfold _bindpi. unfold _retpi. intros.
+      destruct H.
+      + destruct H as [a0 [Hvala0 Hfa0] ].
+        apply eutt_inv_Ret in Hvala0. subst. auto.
+      + exfalso. destruct H. eapply ret_not_div. eauto.
+    - simpl. destruct (f a) as [fa Hfa] eqn : Heq. simpl. intros.
+      left. exists a. split.
+      + reflexivity.
+      + rewrite Heq.  auto.
+  Qed.
+
+  Lemma bindpi_retpi : forall A (w : PureITreeSpec A), (bind w (fun x => ret x) ≈ w)%monad.
+  Proof.
+    intros. destruct w as [ w Hw]. split.
+    - intros. simpl in *. unfold _bindpi in H.
+      unfold _retpi in H. simpl in H.
+      refine (Hw _ _ _ _ _ H).
+      intros. destruct H0.
+      + destruct H0 as [a [ Hvala Hpa]  ].
+        eapply Hp; eauto. symmetry. auto.
+      + destruct H0. apply div_spin_eutt in H0. eapply Hp; eauto.
+    - simpl. intros. unfold _bindpi.
+      refine (Hw _ _ _ _ _ H). intros. unfold _retpi.
+      specialize (eutt_reta_or_div i') as Hor. destruct Hor.
+      + destruct H1 as [a Ha]. left. exists a. split; auto. eapply Hp; eauto.
+      + right. split; auto. specialize (div_spin_eutt H1) as H2. symmetry in H2. eapply Hp; eauto.
+   Qed.
+
+  Lemma bindpi_bindpi : forall (A B C : Type) (w : PureITreeSpec A)
+                               (f : A -> PureITreeSpec B) (g : B -> PureITreeSpec C),
+      (bind (bind w f) g ≈ bind w (fun a => bind (f a) g))%monad.
+  Proof.
+    intros. destruct w as [w Hw]. simpl. split; intros.
+    - simpl in *. refine (Hw _ _ _ _ _ H). intros t0. intros. destruct H0.
+      + destruct H0 as [a [Hreta Hfa]].
+        left. exists a. split; auto. destruct (f a) as [wfa Hwfa]. simpl in *.
+        refine (Hwfa _ _ _ _ _ Hfa). intros t1. intros. destruct H0; auto.
+      + destruct H0. destruct H1.
+        * destruct H1 as [b [Hretb Hgb ]  ]. exfalso. specialize (@ret_not_div B void1 b) as Hndiv.
+          rewrite Hretb in Hndiv. apply Hndiv. apply spin_infinite.
+        *  right. destruct H1. auto.
+    - simpl in *. refine (Hw _ _ _ _ _ H). intros t0. intros. destruct H0.
+      +  destruct H0 as [a [Hreta Hfa] ]. left. exists a. split; auto.
+         destruct (f a) as [wfa Hwfa]. simpl in *.
+         refine (Hwfa _ _ _ _ _ Hfa). intros t1. intros.
+         destruct H0; auto.
+      + destruct H0. right. split; auto. right. split; auto. apply spin_infinite.
+  Qed.
+
+  Instance PureItreeSpecLaws : MonadLawsE PureITreeSpec.
+  Proof.
+    constructor.
+    - apply retpi_bindpi.
+    - apply bindpi_retpi.
+    - apply bindpi_bindpi.
+    - intros. red. red. intros mx my Hxy. red. red. red. intros f g Hfg.
+      intros. red in Hfg. destruct mx as [ mx Hmx]. destruct my as [my Hmy].
+      cbn. unfold _bindpi. do 2 red in Hxy. cbn in Hxy.
+      rewrite Hxy. red in Hmy. split; intros; try refine (Hmy _ _ _ _ _ H); eauto.
+      + intros. cbn in H0. destruct H0; eauto. left.
+        decompose record H0. exists x. split; auto. apply Hfg. auto.
+      + intros. cbn in H0. destruct H0; eauto. left.
+        decompose record H0. exists x. split; auto. apply Hfg. auto.
+  Qed.
+
+
+  Instance PureITreeOrderM : OrderM PureITreeSpec :=
+    fun A (w1 w2 : PureITreeSpec A) => forall p Hp, proj1_sig w2 p Hp -> proj1_sig w1 p Hp.
+
+  Instance PureItreeOrder : OrderedMonad PureITreeSpec.
+  Proof.
+    constructor.
+    - intros. repeat red. intros. destruct w. auto.
+    - intros. repeat red. repeat red in H, H0. intros. destruct w1.
+      destruct w2. destruct w3. simpl in *. auto.
+    - intros. destruct w1 as [w1' Hw1']. destruct w2 as [w2' Hw2']. simpl in *.
+      intros p Hp. simpl.
+      unfold _bindpi. intros.  eapply H. simpl.
+      refine (Hw2' _ _ _ _ _ H1). intros t. intros. destruct H2; auto.
+      destruct H2 as [a [Hreta Hf2a] ]. left. specialize (H0 a p Hp). exists a. auto.
+  Qed.
+(*
+  Instance PureITreeIter : Iter (Kleisli PureITreeSpec) sum := @iterp.
+
+  Instance PureITreeIterUnfold : IterUnfold  (Kleisli PureITreeSpec) sum.
+  Proof.
+    intros A B f a.
+    constructor.
+    (*this case went through without even needing coinduction???*)
+    - intros. red. repeat red in H. punfold H. destruct H.
+      cbn. unfold bindpi, _bindpi. destruct (f a) as [fa Hfa]; simpl in *.
+      eapply Hfa; eauto. intros t ?Ht. inversion Ht; eauto.
+      + left. exists (inr b). split; auto.
+      + left. exists (inl a'). split; auto. pclearbot. auto.
+    (*very suspicious that I no longer need to coinduct, I think I will move this onto a refactor branch to experiment on*)
+    - revert a. (* pcofix CIH. *) intros. cbn in H. pfold. unfold bindpi, _bindpi in H.
+      constructor. destruct (f a) as [fa Hfa]; simpl in *. eapply Hfa; try apply H.
+      intros t ?Ht. simpl in Ht. basic_solve; auto.
+      + eapply cont_a; try apply H0. cbn in H1.
+        red in H1. auto.
+      + eapply term_b; try apply H0. auto.
+  Qed.
+
+  Instance PureITreeIterNatural : IterNatural (Kleisli PureITreeSpec) sum.
+  Proof.
+    intros A B C. intros. constructor.
+    - intros. generalize dependent a. pcofix CIH. intros. pfold. repeat red in H.
+      punfold H0. destruct H0.
+      destruct (f a) as [fa Hfa] eqn : Heq. simpl in *. constructor.
+      cbn. rewrite Heq. simpl. unfold _bindpi. eapply Hfa; eauto.
+      intros t ?Ht. basic_solve.
+      + right. split; auto. apply inf_tau; auto. apply spin_div.
+      + left. exists (inr b). split; auto. cbn. unfold bindpi, _bindpi. simpl.
+        destruct (g b) as [gb Hgb] eqn : Heq'. simpl in *. eapply Hgb; try apply H1. intros ?t ?Ht.
+        clear H. specialize (eutt_reta_or_div C t0) as Hor. basic_solve.
+        * left. exists a0. unfold _retpi. split; auto. eapply term_b; try reflexivity. eapply Hp; eauto.
+        * right. split; auto. eapply inf_tau; try apply spin_div. eapply Hp; eauto. symmetry. apply div_spin_eutt. auto.
+      + left. exists (inl a'). split; auto. cbn. unfold _bindpi, _retpi, id. left. exists a'.
+        split; try reflexivity. eapply cont_a; try reflexivity. right. apply CIH; auto.
+    - intros. generalize dependent a. pcofix CIH. intros. pfold. red.
+      repeat red in H0.
+      constructor.
+      destruct (f a) as [fa Hfa] eqn : Heq. simpl in *. punfold H0. destruct H0. simpl in H.
+      cbn in H. unfold bindpi, _bindpi in H. rewrite Heq in H. simpl in *. eapply Hfa; try apply H.
+      intros t ?. simpl in *. basic_solve.
+      + cbn in H1. unfold _bindpi, _retpi in H1. basic_solve. unfold id in *. basic_solve.
+        eapply cont_a; eauto. auto.
+      + cbn in H1. unfold bindpi, _bindpi in H1. eapply term_b; try apply H0.
+        left. exists b. split; try reflexivity. destruct (g b) as [gb Hgb] eqn : Heq'.
+        simpl in *. eapply Hgb; try apply H1. intros ?t ?Ht. simpl in *. basic_solve.
+        * unfold _retpi in H3. basic_solve. eapply Hp; eauto. symmetry. auto.
+        * apply div_spin_eutt in H2. eapply Hp; eauto.
+      + apply inf_tau; auto. right. split; auto. apply spin_div.
+   Qed.
+
+  (*I am sorry, I will come up for some automation for this eventually*)
+  Instance PureITreeDinatural : IterDinatural (Kleisli PureITreeSpec) sum.
+  Proof.
+    intros A B C. intros. constructor.
+    (* can't coinduct in this case it seems, fingers crossed I don't need to *)
+    - intros. cbn. unfold bindpi, _bindpi. destruct (f a) as [fa Hfa] eqn : Heq. simpl.
+      cbn in H. punfold H. destruct H. cbn in H. unfold bindpi, _bindpi in H. rewrite Heq in H. simpl in *.
+      eapply Hfa; try apply H. intros t ?. simpl in H0.
+      basic_solve; auto.
+      + rename a0 into b. left. exists (inl b). split; auto. cbn. cbn in H1. clear H. clear H0.
+        generalize dependent b. pcofix CIH.
+        intros. pfold. constructor. cbn. unfold bindpi, _bindpi.
+        destruct (g b) as [gb Hgb] eqn : ?Heq. simpl in *. eapply Hgb; try apply H1.
+        intros ?t ?Ht. basic_solve.
+        * right. split; auto. apply inf_tau; auto. apply spin_div.
+        * rename b0 into c. left. exists (inr c). split; auto. cbn. unfold _retpi.
+          eapply term_b; eauto. reflexivity.
+        * left. exists (inl a'). split; auto. cbn. punfold Hcorec. destruct Hcorec. cbn in H.
+          unfold bindpi, _bindpi in H. destruct (f a') as [fa' Hfa'] eqn :?Heq. simpl in *.
+          eapply Hfa'; try apply H. intros ?t ?Ht. simpl in *. basic_solve.
+          -- cbn in H2. rename a0 into b'. eapply cont_a; eauto. auto.
+          -- cbn in H2. rename b0 into c. unfold _retpi in H2. basic_solve.
+             eapply term_b; try apply Hb. auto.
+          -- apply inf_tau; auto.
+      + cbn in H1. unfold _retpi in H1. basic_solve. rename b into c. left.
+        exists (inr c). auto.
+  - intros. generalize dependent a. pcofix CIH.
+    intros. pfold. constructor. cbn. cbn in H0. unfold bindpi, _bindpi in *.
+    destruct (f a) as [fa Hfa] eqn : Heq. simpl in *. eapply Hfa; try apply H0.
+    intros t ?. simpl in *. basic_solve.
+    + rename a0 into b. left. exists (inl b). split; auto. cbn. cbn in H1. red in H1.
+      punfold H1. destruct H1. cbn in H1. unfold bindpi, _bindpi in H1. destruct (g b) as [gb Hgb] eqn : ?Heq.
+      simpl in *. eapply Hgb; try apply H1. intros ?t ?Ht. simpl in *. clear H1.
+      basic_solve.
+      * cbn in H2. eapply cont_a; try apply H1. right. apply CIH. cbn.
+        unfold bindpi, _bindpi. destruct (f a0) as [fa0 Hfa0] eqn : ?Heq. simpl in *.
+        eapply Hfa0; try apply H2. intros ?t ?Ht. basic_solve; auto.
+        -- rename b0 into c. left. exists (inr c). split; auto.
+        -- rename a' into b'. left. exists (inl b'). split; auto.
+      * cbn in H2. unfold _retpi in H2. basic_solve.
+        rename b0 into c. eapply term_b; try apply Hb. auto.
+      * apply inf_tau; auto.
+    + cbn in H1. unfold _retpi, id in H1. left. rename b into c. exists (inr c). split; auto.
+      cbn. unfold _retpi. eapply term_b; eauto. reflexivity.
+    + right. split; auto. apply inf_tau; auto. apply spin_div.
+  Qed.
+
+  Instance PureITreeIterCodiagonal : IterCodiagonal (Kleisli PureITreeSpec) sum.
+  Proof.
+    intros A B f. constructor.
+    - intros. generalize dependent a. pcofix CIH. intros. cbn in H0. punfold H0.
+      pfold. destruct H0. constructor. cbn in H. cbn. punfold H.  destruct H.
+      unfold bindpi, _bindpi. destruct (f a) as [fa Hfa] eqn : Heq. simpl in *. eapply Hfa; try apply H.
+      intros t ?. simpl in *. basic_solve.
+      + right. split; auto.
+      + left. exists (inr (inr b) ). split; auto. clear H. cbn. unfold _retpi.
+        eapply term_b; try apply Hb0. reflexivity.
+      + left. exists (inr (inl a0) ). clear H. split; auto. cbn. unfold _retpi.
+        eapply cont_a; unfold id; try reflexivity. right. apply CIH. apply Hcorec.
+      + left. exists (inl a'). split; auto. cbn. unfold _retpi.
+        eapply cont_a; try reflexivity. clear H. right. apply CIH. red. pfold.
+        red. constructor. punfold Hcorec. red in Hcorec. destruct Hcorec. destruct (f a') as [fa' Hfa'] eqn : ?Heq.
+        simpl in *. red. pfold. constructor. rewrite Heq0. simpl in *.
+        eapply Hfa'; try apply H. clear H. intros ?t ?Ht. auto.
+    - intros. punfold H. generalize dependent a. pcofix CIH. intros. cbn in H0. pfold. constructor.
+      destruct H0. cbn in H. cbn.  unfold bindpi, _bindpi in H. pfold. constructor.
+      destruct (f a) as [fa Hfa] eqn : Heq. simpl in *. eapply Hfa; try apply H.
+      rename H into Ha.
+      intros t ?. simpl in *. basic_solve.
+      + cbn in H0. unfold _retpi in H0. basic_solve. eapply cont_a; try apply H.
+        clear H.  left.
+        generalize dependent a0.
+        pcofix CIH'. intros. pfold. constructor. clear Ha. punfold Hcorec.
+        destruct Hcorec. cbn in H. unfold bindpi, _bindpi in H. simpl in *.
+        destruct (f a0) as [fa0 Hfa0] eqn : ?Heq. simpl in *. eapply Hfa0; try apply H.
+        clear H. intros ?t ?Ht. simpl in *. basic_solve.
+        * cbn in H0. unfold _retpi in H0. basic_solve. eapply cont_a; try apply H. auto.
+        * cbn in H0. unfold _retpi in H0. basic_solve. eapply term_b; try apply H. eapply cont_a; try reflexivity.
+          right. apply CIH. punfold Hcorec.
+        * cbn in H0. unfold _retpi, id in H0. basic_solve. eapply term_b; try apply H.
+          eapply term_b; try reflexivity. auto.
+        * apply inf_tau; auto.
+      + cbn in H0. unfold _retpi, id in H0. basic_solve. eapply term_b; try apply H. eapply cont_a; try reflexivity.
+        right. apply CIH. punfold Hcorec.
+      + cbn in H0. unfold _retpi, id in H0. basic_solve. eapply term_b; try apply H. eapply term_b; try reflexivity.
+        auto.
+      + apply inf_tau; auto.
+   Qed.
+
+
+  Lemma obsip_pres_iter_right : forall A B (f : A -> itree void1 (A + B) ) (a : A)
+            (p : itree void1 B -> Prop) (Hp : resp_eutt void1 B p),
+     proj1_sig (obsip B (iter f a)) p Hp -> proj1_sig (iterp (fun x => obsip _ (f x) ) a) p Hp.
+  Proof.
+    intros. generalize dependent a. pcofix CIH. intros. pfold. constructor.
+    cbn. red.
+    simpl. specialize (unfold_iter_ktree f a) as Hunfold.
+    cbn in H0. red in H0. symmetry in Hunfold. eapply Hp in H0;
+                                                 try (rewrite <- Hunfold; reflexivity).
+    specialize (eutt_reta_or_div _ (f a) ) as [Hret | Hdiv]; basic_solve.
+    - eapply cont_a; try apply Hret. right. apply CIH. cbn. red. eapply Hp; eauto. rewrite <- Hret.
+      setoid_rewrite bind_ret.
+      rewrite tau_eutt. reflexivity.
+    - eapply term_b; try apply Hret. eapply Hp; eauto.
+      rewrite <- Hret. match goal with | |- _ ≈ ITree.bind _ ?g =>
+                              specialize (bind_ret (inr b) g) as Hbind_ret end.
+        rewrite Hbind_ret. reflexivity.
+    - apply div_spin_eutt in Hdiv as Hspin. apply inf_tau; auto.
+      eapply Hp; eauto. rewrite Hspin. apply spin_bind.
+   Qed.
+
+  Ltac proof_by_contra := match goal with | |- ?P => destruct (classic P) as [ ? | Hcontra];
+                                                     auto end.
+
+  Lemma obsip_pres_iter_left : forall A B (f : A -> itree void1 (A + B) ) (a : A)
+                             (p : itree void1 B -> Prop) (Hp : resp_eutt void1 B p),
+      proj1_sig (iterp (fun x => obsip _ (f x) ) a) p Hp -> proj1_sig (obsip B (iter f a)) p Hp.
+  Proof.
+    intros. cbn. red. cbn in H. red in H. cbn in H.
+    punfold H. destruct H. cbn in H. red in H.
+    basic_solve; auto.
+    - apply div_spin_eutt in Ht as H1. eapply Hp; eauto.
+      specialize (unfold_iter_ktree f a) as Hunfold. rewrite Hunfold. rewrite H1.
+      symmetry. apply spin_bind.
+    - specialize (unfold_iter_ktree f a) as Hunfold.
+      eapply Hp; eauto. rewrite Hunfold. rewrite <- Hretb.
+      match goal with | |- ITree.bind _ ?g ≈ _ => specialize (bind_ret (inr b) g)
+      as Hbind_ret end. simpl in *. rewrite Hbind_ret. reflexivity.
+    - specialize (unfold_iter_ktree f a) as Hunfold. eapply Hp; eauto;
+      try (rewrite Hunfold; reflexivity).
+      (* assert (_iter (fun x : A=> obsip (A + B) (f x) ) a'  p Hp); auto. *) unfold resp_eutt in *.
+      eapply Hp with (t1 := KTree.iter f a'); eauto.
+      + rewrite <- Hreta. setoid_rewrite bind_ret.
+        rewrite tau_eutt. reflexivity.
+      + (* I have unfolded in some sense, I want to have a coinductive hyp here *)
+  Abort.
+
+  Lemma iter_too_big_aux : exists A B (f : A -> itree void1 (A + B) ) (p : itree void1 B -> Prop) (a : A) Hp,
+       proj1_sig (iterp (fun x => obsip _ (f x) ) a) p Hp /\ ~ proj1_sig (obsip B (iter f a)) p Hp.
+  Proof.
+    exists nat. exists nat. exists (fun n => ret (inl n) ). exists (fun _ => False).
+    exists 0. assert (resp_eutt _ _ (fun _  : itree void1 nat => False) ).
+    { intros t1 t2. tauto. } exists H.
+    split; auto.
+    pcofix CIH. pfold. constructor. cbn. red. eapply cont_a; eauto. reflexivity.
+  Qed.
+
+  Lemma iter_too_big : ~  forall A B (f : A -> itree void1 (A + B) ) (a : A)
+                             (p : itree void1 B -> Prop) (Hp : resp_eutt void1 B p),
+      proj1_sig (iterp (fun x => obsip _ (f x) ) a) p Hp -> proj1_sig (obsip B (iter f a)) p Hp.
+  Proof.
+    intro Hcontra.
+    specialize iter_too_big_aux as Hlem. basic_solve. auto.
+  Qed.
+
+  (*Other direction is odd, because I can't just straightforwardly coinduct*)
+
+  Lemma obsip_pres_iter : forall A B (f : A -> itree void1 (A + B) ) (a : A),
+        obsip _ (iter f a) ≈ iterp (fun (x : A) => obsip (A + B) (f x) ) a.
+  Proof.
+    intros. constructor.
+    -  apply obsip_pres_iter_right.
+    - intros. cbn. red. cbn in H. unfold obsip, _obsip in H. simpl in H.
+      red in H. punfold H. destruct H. simpl in *.
+      cbn in H.
+  Abort.
+*)
+
+  (*Definition of effect observation from pure itrees into pure itree specs *)
+  Definition _obsip A (t : itree void1 A) : _PureITreeSpec A := fun p _ => p t.
+(*
+  Definition f A : A -> itree void1 nat := fun (a : A) => ret 2.
+
+  Lemma ex : forall p Hp, _obsip nat (bind spin f) p Hp.
+    intros. unfold _obsip. *)
+
+  Lemma obsip_monot : forall A (t : itree void1 A), monotonici A (_obsip A t).
+  Proof.
+    unfold monotonici. intros. unfold _obsip in *. auto.
+  Qed.
+
+  Definition obsip A (t : itree void1 A) : PureITreeSpec A :=
+    exist _ (_obsip A t) (obsip_monot A t).
+
+  (*Proof that this effect observation is a valid monad morphism*)
+  Lemma obsip_pres_ret : forall A (a : A), (obsip A (ret a) ≈ ret a)%monad.
+  Proof.
+    intros. intros p Hp. cbn. unfold _retpi, _obsip. tauto.
+  Qed.
+
+  Lemma obsip_pres_bind : forall A B (t : itree void1 A) (f : A -> itree void1 B),
+        (obsip B (bind t f) ≈ bind (obsip A t) (fun a => obsip B (f a)))%monad.
+  Proof.
+    intros. intros p Hp. cbn. unfold _obsip, _bindpi. split; intros.
+    - specialize (eutt_reta_or_div t) as Hor. destruct Hor.
+      + destruct H0 as [a Hreta ]. left. exists a. split; auto.
+        eapply Hp; eauto. specialize (bind_ret_l a f) as H1. rewrite <- H1.
+        rewrite Hreta. reflexivity.
+      + right. split; auto. apply div_spin_eutt in H0. rewrite (spin_bind f), <- H0; apply H.
+    - destruct H.
+      + destruct H as [a [Hreta Hpfa] ]. specialize (bind_ret_l a f) as H1.
+        eapply Hp; eauto.  rewrite <- H1. rewrite Hreta. reflexivity.
+      + destruct H. apply div_spin_eutt in H.
+        rewrite H, <- spin_bind. apply H0.
+  Qed.
+
+  Lemma obsip_eutt : forall A (t1 t2 : itree void1 A), t1 ≈ t2 <-> (obsip A t1 ≈ obsip A t2)%monad.
+  Proof.
+    split; intros; unfold obsip, _obsip in *; simpl in *.
+    - intros p Hp. simpl. split; intros; eapply Hp; eauto.
+      symmetry. auto.
+    - set (fun t => t ≈ t1) as p.
+      assert (Hp : resp_eutt p).
+      + intros t3 t4. unfold p. split; intros.
+        * rewrite <- H1. symmetry. auto.
+        * rewrite H0. auto.
+      + specialize (H p Hp). simpl in *. unfold p in H. symmetry. apply H. reflexivity.
+  Qed.
+
+  #[global] Instance PureITreeEffectObs : EffectObs (itree void1) (PureITreeSpec) := obsip.
+
+  #[global] Instance PureITreeMorph : MonadMorphism (itree void1) (PureITreeSpec) PureITreeEffectObs.
+  Proof.
+    constructor.
+    - apply obsip_pres_ret.
+    - apply obsip_pres_bind.
+  Qed.
+
+End PureITree.
