src/ItreeExtra/Dijkstra/StateDelaySpec.v
@@ -1,0 +1,255 @@
+From ExtLib Require Import
+     Data.List
+     Structures.Monad.
+
+From Paco Require Import paco.
+
+From ITree Require Import
+     ITree
+     ITreeFacts
+     Events.MapDefault
+     Events.State
+     Events.StateFacts.
+
+From ITree.Extra Require Import
+     Dijkstra.DijkstraMonad
+     Dijkstra.PureITreeBasics
+     Dijkstra.DelaySpecMonad
+     Dijkstra.StateSpecT.
+
+Import Monads.
+Import MonadNotation.
+#[local] Open Scope monad_scope.
+#[local] Open Scope delayspec_scope.
+
+(* Defines a specification monad for the state transform of the Delay monad. Also includes encodings for pre post condition specifications. *)
+
+Section StateDelaySpec.
+
+  Context (St : Type).
+
+  Definition StateDelaySpec := StateSpecT St DelaySpec.
+
+  Definition StateDelaySpecOrder := StateSpecTOrder St DelaySpec.
+
+  Definition StateDelaySpecOrderedLaws := StateSpecTOrderedLaws St DelaySpec.
+
+  Definition StateDelaySpecEq := StateSpecTEq St DelaySpec.
+
+  Definition StateDelaySpecMonadLaws := StateSpecTMonadLaws St DelaySpec.
+
+  Definition StateDelay := StateSpecT St Delay.
+
+  Definition StateDelayObs := EffectObsStateT St DelaySpec Delay.
+
+  Definition StateDelayMonadMorph := MonadMorphimStateT St DelaySpec Delay.
+
+  Definition PrePost A : Type := (Delay (St * A) -> Prop ) * (St -> Prop).
+
+  Definition PrePostRef {A : Type} (m : StateDelay A) (pp : PrePost A) : Prop :=
+    let '(post,pre) := pp in
+    forall s, pre s -> post (m s).
+
+  Program Definition encode {A : Type} (pp : PrePost A) : StateDelaySpec A :=
+    let '(post,pre) := pp in
+    fun s p => pre s /\ (forall r, post r -> p r).
+
+  Definition verify_cond {A : Type} := DijkstraProp StateDelay StateDelaySpec StateDelayObs A.
+
+  Lemma encode_correct : forall (A : Type) (pre : St -> Prop) (post : Delay (St * A) -> Prop)
+                                (m : StateDelay A),
+      resp_eutt post -> (PrePostRef m (post,pre) <-> verify_cond (encode (post,pre)) m).
+  Proof.
+    intros. cbn. unfold verify_cond, DijkstraProp.
+    split; intros.
+    - repeat red. simpl. intros. destruct p as [p Hp]. simpl in H1. destruct H1 as [Hpre Himp].
+      auto.
+    - repeat red in H0. simpl in H0.
+      set (exist _ post H) as p. enough ((m s) ∈ p); auto.
+      apply H0. auto.
+  Qed.
+
+  Definition PrePostPair A : Type := PrePost A * PrePost A.
+
+  Definition PrePostPairRef {A : Type} (pppp : PrePostPair A) (m : StateDelay A) :=
+    let '((post0, pre0), (post1, pre1)) := pppp in
+    forall s, (pre0 s -> post0 (m s)) /\ (pre1 s -> post1 (m s)) .
+
+  Program Definition encode_pair {A : Type} (pppp : PrePostPair A) : StateDelaySpec A:=
+    let '((post0, pre0), (post1, pre1)) := pppp in
+    fun s (p : DelaySpecInput (St * A)) =>
+      (pre0 s /\ (forall r, post0 r -> p r)) \/ (pre1 s /\ forall r, post1 r -> p r).
+  Next Obligation.
+  destruct H0 as [H0 | H1].
+  - destruct H0 as [Hp Hr]. left. auto.
+  - destruct H1 as [Hp Hr]. right. auto.
+  Qed.
+
+  Lemma encode_pair_correct : forall (A : Type) (pre0 pre1 : St -> Prop)
+                                          (post0 post1 : Delay (St * A) -> Prop ) (m : StateDelay A),
+      let pp : PrePostPair A := ((post0,pre0),(post1,pre1)) in
+      resp_eutt post0 -> resp_eutt post1 ->
+      (PrePostPairRef pp m <-> verify_cond (encode_pair pp) m).
+  Proof.
+    intros. cbn. unfold verify_cond, DijkstraProp. split; intros.
+    - repeat red. simpl. intros. destruct p as [p Hrp].
+      specialize (H1 s). destruct H1.
+      destruct H2 as [ [Hs Hp] | [Hs Hp]  ]; simpl in *; auto.
+    - repeat red in H1. simpl in *.
+      split; intros.
+      + set (exist _ post0 H) as p. enough ((m s) ∈ p ); auto.
+        apply H1. left. split; auto.
+      + set (exist _ post1 H0) as p. enough ((m s) ∈ p ); auto.
+        apply H1. right. split; auto.
+  Qed.
+
+  Definition PrePostList A : Type := list (PrePost A).
+
+  Definition PrePostListRef {A : Type} (ppl : PrePostList A) (m : StateDelay A) :=
+    forall s, List.Forall (fun pp : PrePost A=> let (post,pre) := pp in pre s -> post (m s) ) ppl.
+
+  Program Definition encode_list {A : Type} (ppl : PrePostList A) : StateDelaySpec A :=
+    fun s (p : DelaySpecInput (St * A) ) =>
+      List.Exists (fun pp : PrePost A => let (post,pre) := pp in pre s /\ forall r, post r -> p r) ppl.
+  Next Obligation.
+    induction H0; eauto.
+    destruct x as [post pre]. destruct H0 as [Hs Hr]. left. auto.
+  Qed.
+
+
+  Lemma enocde_list_correct : forall (A : Type) (ppl : PrePostList A) (m : StateDelay A),
+      List.Forall (fun pp => resp_eutt (fst pp) ) ppl->
+      (PrePostListRef ppl m <-> verify_cond (encode_list ppl) m).
+  Proof.
+    intros. unfold verify_cond, DijkstraProp. split; intros.
+    - repeat red. intros. destruct p as [p Hp]. red in H0.
+      specialize (H0 s) as Hrefine. unfold encode_list in H1. simpl in *.
+      induction ppl.
+      + inversion H1.
+      + destruct a as [post pre].
+        inversion H1; subst.
+        * destruct H3. auto.
+          assert ((pre s -> post (m s)) ); auto.
+          intros. inversion Hrefine; subst; auto.
+        * apply IHppl; auto.
+          -- inversion H; auto.
+          -- intros. specialize (H0 s0). inversion H0. auto.
+          -- specialize (H0 s). inversion H0. auto.
+    - unfold encode_list in H0. simpl in *. repeat red. repeat red in H0. simpl in *. intros.
+      induction ppl; auto.
+      destruct a as [post pre]. specialize (H0 s) as Henc.
+      assert (Heutt : resp_eutt post).
+      { inversion H. auto. }
+      set (exist _ post Heutt) as p. specialize (Henc p) as Hencp.
+      constructor; intros.
+      + enough ((m s) ∈ p ); auto. apply Hencp.
+        left. split; auto.
+      + apply IHppl; auto.
+        * inversion H. auto.
+        * clear IHppl. intros. apply H0. eauto.
+  Qed.
+
+  Definition DynPrePost A : Type := (St -> Prop) * (St -> Delay (St * A) -> Prop).
+
+  Definition DynPrePostRef {A : Type} (pp : DynPrePost A) (m : StateDelay A) :=
+    let (pre,post) := pp in
+    forall s, pre s -> post s (m s).
+
+  Program Definition encode_dyn {A : Type} (pp : DynPrePost A) : StateDelaySpec A :=
+    let (pre,post) := pp in
+    fun s p => pre s /\ forall r, post s r -> p r.
+
+  Lemma encode_dyn_correct : forall (A : Type) (pre : St -> Prop) (post : St -> Delay (St * A) -> Prop ) (m : StateDelay A),
+      (forall s, resp_eutt (post s)) -> (DynPrePostRef (pre,post) m <-> verify_cond (encode_dyn (pre,post) ) m).
+    Proof.
+      intros. unfold verify_cond, DijkstraProp. split; intros.
+      - repeat red. red in H0. intros. destruct p as [p Hp]. simpl in *.
+        destruct H1 as [Hs Hr]. auto.
+      - repeat red in H0. red. intros.
+        set (exist _ (post s) (H s) ) as p. specialize (H0 s p).
+        unfold p in H0. simpl in *. auto.
+    Qed.
+
+  Definition DynPrePostListRef {A : Type} (ppl : list (DynPrePost A)) (m : StateDelay A) : Prop :=
+    Forall (fun pp => DynPrePostRef pp m) ppl.
+
+  Program Definition encode_list_dyn {A : Type} (ppl : list (DynPrePost A)) : StateDelaySpec A :=
+    fun s p => List.Exists (fun pp : DynPrePost A => let (pre,post) := pp in pre s /\ forall r, post s r -> p r ) ppl.
+  Next Obligation.
+    induction H0; eauto. left. destruct x as [pre post]. destruct H0 as [Hs Hr].
+    split; auto.
+  Qed.
+
+  Lemma enocde_list_dyn_correct : forall (A : Type) (ppl : list (DynPrePost A) ) (m : StateDelay A),
+      List.Forall (fun pp => forall s, resp_eutt (snd pp s) ) ppl->
+      (DynPrePostListRef ppl m <-> verify_cond (encode_list_dyn ppl) m).
+  Proof.
+    intros. unfold verify_cond, DijkstraProp. split; intros.
+    - repeat red. intros. destruct p as [p Hp]. simpl in H1. red in H0. rename H0 into Hrefine.
+      unfold DynPrePostRef in Hrefine.
+      induction ppl.
+      + inversion H1.
+      + destruct a as [pre post].
+        inversion H1; subst.
+        * destruct H2.
+          assert ((pre s -> post s (m s)) ); auto.
+          intros. inversion Hrefine; subst; auto.
+        * apply IHppl; auto.
+          -- inversion H; auto.
+          -- intros. inversion Hrefine; auto.
+    - unfold encode_list in H0. simpl in *. repeat red. repeat red in H0. simpl in *. intros.
+      induction ppl; auto.
+      destruct a as [pre post].
+      assert (Heutt : forall s, resp_eutt (post s)).
+      { inversion H. auto. }
+      constructor; intros.
+      + red. intros. set (exist _ (post s) (Heutt s)) as p.
+        specialize (H0 s p). enough ((m s) ∈ p); auto. apply H0.
+        left. split; auto.
+      + apply IHppl; auto.
+        * inversion H. auto.
+        * clear IHppl. intros.
+          specialize (H0 s p). apply H0. eauto.
+  Qed.
+
+  Lemma combine_prepost_aux : forall (A B : Type) (pre1 pre2 : St -> Prop)
+                (post1 : Delay (St * A) -> Prop ) (post2 : Delay (St * B) -> Prop)
+    (m : StateDelay A) (f : A -> StateDelay B),
+    verify_cond (encode (post1,pre1) ) m ->
+    (forall (a : A) (s : St), (* this condition is not exactly what i want*)
+        post1 (Ret (s,a) ) -> post2 (f a s) ) ->
+    (post1 ITree.spin -> post2 ITree.spin) ->
+    resp_eutt post1 ->
+    verify_cond (encode (post2, pre1) ) (bind m f).
+  Proof.
+    intros. repeat red in H. repeat red. intros.
+    destruct p as [p Hp]. simpl in *.
+    destruct H3.
+    destruct (eutt_reta_or_div (m s)); basic_solve.
+    - destruct a as [s' a].
+      cbn in H5. rewrite <- H5, bind_ret_l; cbn. apply H4, H0. rewrite H5.
+      apply (H s (exist _ post1 H2)); auto.
+    - apply div_spin_eutt in H5.
+      rewrite H5, <- spin_bind. apply H4, H1. rewrite <- H5. apply (H s (exist _ post1 H2)); auto.
+  Qed.
+
+  Lemma combine_prepost : forall (A B : Type) (pre1 pre2 : St -> Prop)
+                (post1 : Delay (St * A) -> Prop ) (post2 : Delay (St * B) -> Prop)
+    (m : StateDelay A) (f : A -> StateDelay B),
+    verify_cond (encode (post1,pre1) ) m ->
+    (forall a s, post1 (Ret (s,a)) -> pre2 s)  ->
+    (forall a, verify_cond (encode (post2,pre2) ) (f a)  ) ->
+    (post1 ITree.spin -> post2 ITree.spin) ->
+    resp_eutt post1 ->
+    resp_eutt post2 ->
+    verify_cond (encode (post2, pre1) ) (bind m f).
+  Proof.
+    intros.
+    eapply combine_prepost_aux; eauto.
+    intros.
+    specialize (H1 a) as Hpp2. repeat red in Hpp2.
+    specialize (Hpp2 s (exist _ post2 H4) ). simpl in *.
+    apply Hpp2. split; eauto.
+  Qed.
+
+End StateDelaySpec.
