src/ItreeExtra/ITrace/ITraceDefinition.v
@@ -1,0 +1,64 @@
+From ITree Require Import
+     ITree
+     ITreeFacts
+     Eq.Rutt
+     Props.Infinite
+.
+
+
+From Paco Require Import paco.
+
+Import Monads.
+Import MonadNotation.
+Local Open Scope monad_scope.
+
+Variant EvAns (E : Type -> Type) : Type -> Type :=
+  | evans : forall {A : Type} (ev : E A) (ans : A), EvAns E unit
+  (*if you can prove there is no answers, don't need to proved one*)
+  | evempty : forall {A : Type} (Hempty : A -> void) (ev : E A), EvAns E void
+.
+
+Arguments evans {E}.
+Arguments evempty {E}.
+
+Definition itrace (E : Type -> Type) (R : Type) := itree (EvAns E) R.
+
+Definition itrace' (E : Type -> Type) (R : Type) := itree' (EvAns E) R.
+
+Definition ev_stream (E : Type -> Type) := itrace E unit.
+
+Definition Nil {E : Type -> Type} : ev_stream E := Ret tt.
+
+Definition ev_list (E : Type -> Type) := list (EvAns E unit).
+
+Fixpoint ev_list_to_stream {E : Type -> Type} (l : ev_list E) : ev_stream E :=
+  match l with
+  | nil => Ret tt
+  | cons e t => Vis e (fun _ => ev_list_to_stream t) end.
+
+(*one append for traces and streams, get associativity for free from bind_bind*)
+Definition append {E R} (s : itrace E unit) (b : itrace E R) :=
+  ITree.bind s (fun _ => b).
+
+Notation "s ++ b" := (append s b).
+
+Variant REvRef (E : Type -> Type) : forall (A B : Type), EvAns E A -> E B -> Prop :=
+  | rer {A : Type} (e : E A) (a : A) : REvRef E unit A (evans A e a) e
+  | ree {A : Type} (e : E A) (Hempty : A -> void) : REvRef E void A (evempty A Hempty e) e
+.
+#[global] Hint Constructors REvRef : itree.
+
+(*shouldn't need an empty case*)
+Variant RAnsRef (E : Type -> Type) : forall (A B : Type), EvAns E A -> A -> E B -> B -> Prop :=
+  | rar {A : Type} (e : E A) (a : A) : RAnsRef E unit A (evans A e a) tt e a.
+#[global] Hint Constructors RAnsRef : itree.
+
+Definition trace_refine {E R}  (t : itree E R) (b : itrace E R)  :=
+   rutt (REvRef E) (RAnsRef E) eq b t.
+
+
+Notation "b ⊑ t" := (trace_refine t b) (at level 70).
+
+Definition finite {E : Type -> Type} (s : ev_stream E) : Prop := may_converge tt s.
+
+#[global] Instance itrace_eq {E} : Eq1 (itrace E) := ITreeMonad.Eq1_ITree.
