src/ItreeExtra/Secure/SecureEqBind.v
@@ -1,0 +1,283 @@
+From ITree Require Import
+     Axioms
+     ITree
+     ITreeFacts.
+
+From ITree.Extra Require Import
+     Secure.SecureEqHalt
+     Secure.SecureEqWcompat
+.
+
+From Paco Require Import paco.
+
+Import Monads.
+Import MonadNotation.
+Local Open Scope monad_scope.
+
+Lemma eqit_bind_shalt_aux1:
+  forall (E : Type -> Type) (S2 S1 R1 R2 : Type) (RR : R1 -> R2 -> Prop)
+    (RS : S1 -> S2 -> Prop) (b1 b2 : bool) (Label : Preorder)
+    (priv : forall A : Type, E A -> L) (l : L) (k1 : R1 -> itree E S1)
+    (k2 : R2 -> itree E S2) (A : Type) (e : E A) (k0 : A -> itree E R1)
+    (t2 : itree E R2),
+    ~ leq (priv A e) l ->
+    empty A ->
+    paco2 (secure_eqit_ Label priv RR b1 b2 l id) bot2 (Vis e k0) t2 ->
+    forall (t1 : itree E R1),
+      VisF e k0 = observe t1 ->
+      paco2 (secure_eqit_ Label priv RS b1 b2 l id) bot2 (ITree.bind t1 k1) (ITree.bind t2 k2).
+Proof.
+  intros E S2 S1 R1 R2 RR RS b1 b2 Label priv l k1 k2 A e k0 t2 SECCHECK SIZECHECK H0 t1 Heqot1.
+  pstep. red. unfold ITree.bind at 1, observe at 1. cbn. rewrite <- Heqot1.
+  cbn. rewrite itree_eta' at 1. pstep_reverse.
+  generalize dependent t2. pcofix CIH. intros t2 Ht2.
+  pstep. red.
+  punfold Ht2. red in Ht2.
+  unfold ITree.bind at 1. unfold observe at 2. cbn in *.
+  inv Ht2; ddestruction; subst; try contra_size; try contradiction; try rewrite <- H; cbn;
+  try unpriv_halt; right; eapply CIH;  pclearbot; eauto;
+  try (pfold; rewrite H in H1; apply H1).
+  contra_size.
+Qed.
+
+Lemma eqit_bind_shalt_aux2:
+  forall (E : Type -> Type) (S2 S1 R1 R2 : Type) (RR : R1 -> R2 -> Prop)
+    (RS : S1 -> S2 -> Prop) (b1 b2 : bool) (Label : Preorder)
+    (priv : forall A : Type, E A -> L) (l : L) (k1 : R1 -> itree E S1)
+    (k2 : R2 -> itree E S2) (A : Type) (e : E A) (k0 : A -> itree E R2)
+    (t1 : itree E R1) (t2 : itree E R2),
+    ~ leq (priv A e) l ->
+    empty A ->
+    paco2 (secure_eqit_ Label priv RR b1 b2 l id) bot2 t1 (Vis e k0) ->
+    VisF e k0 = observe t2 ->
+    paco2 (secure_eqit_ Label priv RS b1 b2 l id) bot2 (ITree.bind t1 k1) (ITree.bind t2 k2).
+Proof.
+  intros E S2 S1 R1 R2 RR RS b1 b2 Label priv l k1 k2 A e k0 t1 t2 SECCHECK SIZECHECK H0 Heqot1.
+  pstep. red. unfold ITree.bind at 2, observe at 2. cbn. rewrite <- Heqot1.
+  cbn. rewrite itree_eta'. pstep_reverse.
+  generalize dependent t1. pcofix CIH. intros t1 Ht1.
+  pstep. red.
+  punfold Ht1. red in Ht1.
+  unfold ITree.bind at 1, observe at 1. cbn in *.
+  inv Ht1; ddestruction; subst; try contra_size; try contradiction; cbn;
+  try unpriv_halt; try contra_size; try (right; eapply CIH; pclearbot; eauto).
+  pfold. rewrite H0 in H1. auto. apply H1.
+Qed.
+
+Lemma secure_eqit_bind' : forall E R1 R2 S1 S2 (RR : R1 -> R2 -> Prop) (RS : S1 -> S2 -> Prop)
+                           b1 b2 Label priv l r
+    (t1 : itree E R1) (t2 : itree E R2) (k1 : R1 -> itree E S1) (k2 : R2 -> itree E S2),
+    (forall r1 r2, RR r1 r2 -> paco2 (secure_eqit_ Label priv RS b1 b2 l id) r (k1 r1) (k2 r2) ) ->
+    eqit_secure Label priv RR b1 b2 l t1 t2 ->
+    paco2 (secure_eqit_ Label priv RS b1 b2 l id) r (ITree.bind t1 k1) (ITree.bind t2 k2).
+Proof.
+  intros. revert H0. revert t1 t2. pcofix CIH. intros t1 t2 Ht12.
+  punfold Ht12. red in Ht12.
+  genobs t1 ot1. genobs t2 ot2.
+  hinduction Ht12 before r; intros; eauto.
+  - pstep. red. unfold ITree.bind, observe. unfold observe. cbn.
+    rewrite <- Heqot1. rewrite <- Heqot2. pstep_reverse.
+    eapply paco2_mon; eauto.
+  - pstep. red. unfold ITree.bind, observe. unfold observe. cbn.
+    rewrite <- Heqot1. rewrite <- Heqot2. cbn. constructor. right. eapply CIH. pclearbot.
+    auto.
+  - pstep. red. unfold ITree.bind at 1, observe at 1. cbn.
+    rewrite <- Heqot1. cbn. constructor; auto. pstep_reverse.
+  - pstep. red. unfold ITree.bind at 2, observe at 2. cbn.
+    rewrite <- Heqot2. cbn. constructor; auto. pstep_reverse.
+  - pstep. red. unfold ITree.bind, observe. unfold observe. cbn.
+    rewrite <- Heqot1. rewrite <- Heqot2. cbn. pclearbot.
+    constructor; auto. right. eapply CIH; eauto. apply H.
+  - pstep. red. unfold ITree.bind, observe. unfold observe. cbn.
+    rewrite <- Heqot1. rewrite <- Heqot2. cbn. unpriv_co.
+    right. pclearbot. eapply CIH; apply H.
+  - pstep. red. unfold ITree.bind, observe. unfold observe. cbn.
+    rewrite <- Heqot1. rewrite <- Heqot2. cbn. unpriv_co.
+    right. pclearbot. eapply CIH; apply H.
+  - pstep. red. unfold ITree.bind, observe. unfold observe. cbn.
+    rewrite <- Heqot1. rewrite <- Heqot2. cbn. unpriv_co.
+    right. pclearbot. eapply CIH; apply H.
+  - pstep. red. unfold ITree.bind at 1, observe at 1. cbn.
+    rewrite <- Heqot1. cbn. unpriv_ind. pstep_reverse; try eapply H0; eauto.
+  - pstep. red. unfold ITree.bind at 2, observe at 2. cbn.
+    rewrite <- Heqot2. cbn. unpriv_ind. pstep_reverse; try eapply H0; eauto.
+  - pclearbot.
+    eapply paco2_mon with (r := bot2); intros; try contradiction.
+    eapply eqit_bind_shalt_aux1; eauto. pfold. red. rewrite <- Heqot2.
+    cbn. unpriv_halt. left. eauto.
+  - pclearbot.
+    eapply paco2_mon with (r := bot2); intros; try contradiction.
+    eapply eqit_bind_shalt_aux2; eauto. pfold. red. cbn. rewrite <- Heqot1.
+    unpriv_halt. left. eauto.
+  - pclearbot.
+    eapply paco2_mon with (r := bot2); intros; try contradiction.
+    eapply eqit_bind_shalt_aux1 with (A := A); eauto.
+    pfold. red. rewrite <- Heqot2. cbn. unpriv_halt.
+  - pclearbot.
+    eapply paco2_mon with (r := bot2); intros; try contradiction.
+    eapply eqit_bind_shalt_aux2; eauto. pfold. red. cbn. rewrite <- Heqot1.
+    unpriv_halt.
+Qed.
+
+Lemma secure_eqit_bind : forall E R1 R2 S1 S2 (RR : R1 -> R2 -> Prop) (RS : S1 -> S2 -> Prop)
+                           b1 b2 Label priv l
+    (t1 : itree E R1) (t2 : itree E R2) (k1 : R1 -> itree E S1) (k2 : R2 -> itree E S2),
+    (forall r1 r2, RR r1 r2 -> eqit_secure Label priv RS b1 b2 l (k1 r1) (k2 r2) ) ->
+    eqit_secure Label priv RR b1 b2 l t1 t2 ->
+    eqit_secure Label priv RS b1 b2 l (ITree.bind t1 k1) (ITree.bind t2 k2).
+Proof.
+  intros.
+  eapply secure_eqit_bind'; eauto.
+Qed.
+
+Lemma iter_bind_shalt_aux1:
+  forall (E : Type -> Type) (B2 B1 A1 A2 : Type) (RA : A1 -> A2 -> Prop)
+    (RB : B1 -> B2 -> Prop) (b1 b2 : bool) (Label : Preorder)
+    (priv : forall A : Type, E A -> L) (l : L) (body1 : A1 -> itree E (A1 + B1))
+    (body2 : A2 -> itree E (A2 + B2)) (r : itree E B1 -> itree E B2 -> Prop)
+    (A : Type) (e : E A) (k1 : A -> itree E (A1 + B1)) (t0 : itree E (A2 + B2)),
+    ~ leq (priv A e) l ->
+    empty A ->
+    paco2 (secure_eqit_ Label priv (HeterogeneousRelations.sum_rel RA RB) b1 b2 l id) bot2
+          (Vis e k1) t0 ->
+    paco2 (secure_eqit_ Label priv RB b1 b2 l id) r
+          (Vis e
+               (fun x : A =>
+                  ITree.bind (k1 x)
+                             (fun lr : A1 + B1 =>
+                                match lr with
+                                | inl l0 => Tau (ITree.iter body1 l0)
+                                | inr r0 => Ret r0
+                                end)))
+          (ITree.bind t0
+                      (fun lr : A2 + B2 =>
+                         match lr with
+                         | inl l0 => Tau (ITree.iter body2 l0)
+                         | inr r0 => Ret r0
+                         end)).
+Proof.
+  intros E B2 B1 A1 A2 RA RB b1 b2 Label priv l body1 body2 r A e k1 t0 SECCHECK SIZECHECK H.
+  generalize dependent t0. pcofix CIH. intros t0 Ht0.
+  pstep. red. cbn. unfold observe. cbn. punfold Ht0.
+  red in Ht0. cbn in *. inv Ht0; inv_vis_secure; cbn; pclearbot; unpriv_halt; try contra_size;
+    right; eauto.
+  eapply CIH; eauto.
+  rewrite H in H1. pfold. red. auto.
+Qed.
+
+Lemma iter_bind_shalt_aux2:
+  forall (E : Type -> Type) (B2 B1 A1 A2 : Type) (RA : A1 -> A2 -> Prop)
+    (RB : B1 -> B2 -> Prop) (b1 b2 : bool) (Label : Preorder)
+    (priv : forall A : Type, E A -> L) (l : L) (body1 : A1 -> itree E (A1 + B1))
+    (body2 : A2 -> itree E (A2 + B2)) (r : itree E B1 -> itree E B2 -> Prop)
+    (A : Type) (e : E A) (t0 : itree E (A1 + B1)) (k2 : A -> itree E (A2 + B2)),
+    ~ leq (priv A e) l ->
+    empty A ->
+    paco2 (secure_eqit_ Label priv (HeterogeneousRelations.sum_rel RA RB) b1 b2 l id) bot2 t0
+          (Vis e k2) ->
+    paco2 (secure_eqit_ Label priv RB b1 b2 l id) r
+          (ITree.bind t0
+                      (fun lr : A1 + B1 =>
+                         match lr with
+                         | inl l0 => Tau (ITree.iter body1 l0)
+                         | inr r0 => Ret r0
+                         end))
+          (Vis e
+               (fun x : A =>
+                  ITree.bind (k2 x)
+                             (fun lr : A2 + B2 =>
+                                match lr with
+                                | inl l0 => Tau (ITree.iter body2 l0)
+                                | inr r0 => Ret r0
+                                end))).
+Proof.
+  intros E B2 B1 A1 A2 RA RB b1 b2 Label priv l body1 body2 r A e t0 k2 SECCHECK SIZECHECK H.
+  generalize dependent t0. pcofix CIH. intros t0 Ht0.
+  pstep. red. cbn. unfold observe. cbn. punfold Ht0.
+  red in Ht0. cbn in *. inv Ht0; inv_vis_secure; cbn; pclearbot; unpriv_halt; try contra_size;
+  try (right; eauto).
+  eapply CIH; eauto.
+  rewrite H0 in H1. pfold. red. auto.
+Qed.
+
+Lemma iter_bind_aux:
+  forall (E : Type -> Type) (B2 B1 A1 A2 : Type) (RA : A1 -> A2 -> Prop)
+    (RB : B1 -> B2 -> Prop) (b1 b2 : bool) (Label : Preorder)
+    (priv : forall A : Type, E A -> L) (l : L) (body1 : A1 -> itree E (A1 + B1))
+    (body2 : A2 -> itree E (A2 + B2)) (r : itree E B1 -> itree E B2 -> Prop)
+    (t1 : itree E (A1 + B1)) (t2 : itree E (A2 + B2)),
+    paco2 (secure_eqit_ Label priv (HeterogeneousRelations.sum_rel RA RB) b1 b2 l id) bot2 t1 t2 ->
+    (forall (a1 : A1) (a2 : A2), RA a1 a2 -> r (ITree.iter body1 a1) (ITree.iter body2 a2)) ->
+    paco2 (secure_eqit_ Label priv RB b1 b2 l id) r
+          (ITree.bind t1
+                      (fun lr : A1 + B1 =>
+                         match lr with
+                         | inl l0 => Tau (ITree.iter body1 l0)
+                         | inr r0 => Ret r0
+                         end))
+          (ITree.bind t2
+                      (fun lr : A2 + B2 =>
+                         match lr with
+                         | inl l0 => Tau (ITree.iter body2 l0)
+                         | inr r0 => Ret r0
+                         end)).
+Proof.
+  intros E B2 B1 A1 A2 RA RB b1 b2 Label priv l body1 body2 r t1 t2 H CIH0.
+  generalize dependent t2. revert t1. pcofix CIH1.
+  intros t1 t2 Ht12. punfold Ht12. pstep. red.
+  unfold observe. cbn.
+  hinduction Ht12 before r; intros; cbn; eauto; pclearbot;
+  try (unpriv_co; fail);
+  try (constructor; auto; pclearbot; right; eapply CIH1; eauto with itree; fail).
+  - inv H; cbn; eauto with itree.
+  - unpriv_ind. unfold observe at 1. cbn. eapply H0; eauto with itree.
+  - unpriv_ind. unfold observe at 3. cbn. eapply H0; eauto with itree.
+  - unpriv_halt. left. eapply iter_bind_shalt_aux1; eauto with itree.
+  - unpriv_halt. left. eapply iter_bind_shalt_aux2; eauto with itree.
+  - unpriv_halt. specialize (H b). left. eapply iter_bind_shalt_aux1; eauto with itree.
+  - unpriv_halt. specialize (H a). left. eapply iter_bind_shalt_aux2; eauto with itree.
+Qed.
+
+
+Lemma secure_eqit_iter : forall E A1 A2 B1 B2 (RA : A1 -> A2 -> Prop) (RB : B1 -> B2 -> Prop)
+                           b1 b2 Label priv l
+                           (body1 : A1 -> itree E (A1 + B1) ) (body2 : A2 -> itree E (A2 + B2) )
+                           (a1 : A1) (a2 : A2),
+    RA a1 a2 ->
+    (forall a1 a2, RA a1 a2 -> eqit_secure Label priv (HeterogeneousRelations.sum_rel RA RB) b1 b2 l (body1 a1) (body2 a2) ) ->
+    eqit_secure Label priv RB b1 b2 l (ITree.iter body1 a1) (ITree.iter body2 a2).
+Proof.
+  intros. rename H0 into Hbody. generalize dependent a2. revert a1.
+  (* gcofix CIH. intros. setoid_rewrite unfold_iter.
+  guclo eqit_bind_clo. *)
+
+  (* look into the more general secure_eqitC closure, see if that is weakly compatible, *)
+  pcofix CIH.
+  intros a1 a2 Ha. specialize (Hbody a1 a2 Ha) as Hbodya.
+  punfold Hbodya. red in Hbodya. pfold. red.
+  unfold observe. (* write lemmas for unfolding the observe of iter *) cbn.
+  hinduction Hbodya before r; intros; cbn; auto with itree.
+  - inv H; cbn; eauto with itree.
+  - cbn. pclearbot. constructor.
+    left. eapply iter_bind_aux; eauto.
+  - constructor; auto. pclearbot. left. eapply iter_bind_aux; eauto.
+  - unpriv_co. pclearbot. left. eapply iter_bind_aux; eauto.
+  -  unpriv_co. pclearbot. left. eapply iter_bind_aux; eauto.
+  - unpriv_co. pclearbot. left. eapply iter_bind_aux; eauto.
+  - unpriv_ind. (* here is  where it gets bad, I am pretty sure H0 does match up but could
+                  take very particular *) unfold observe at 1. cbn.
+    eauto.
+  - unpriv_ind. unfold observe at 3. cbn. eauto.
+  - pclearbot. unpriv_halt.
+    left. eapply iter_bind_shalt_aux1; eauto.
+  - unpriv_halt. pclearbot. left. eapply iter_bind_shalt_aux2; eauto.
+  - unpriv_halt. pclearbot. specialize (H b). left.
+    eapply iter_bind_shalt_aux1; eauto.
+  - unpriv_halt. pclearbot. specialize (H a). left. eapply iter_bind_shalt_aux2; eauto.
+Qed.
+
+Lemma secure_eqit_ret : forall (E : Type -> Type) Label priv l b1 b2 (R1 R2 : Type) (RR : R1 -> R2 -> Prop) (r1 : R1) (r2 : R2),
+    RR r1 r2 -> @eqit_secure E R1 R2 Label priv RR b1 b2 l (Ret r1) (Ret r2).
+Proof.
+  intros. pfold. constructor. auto.
+Qed.
