src/ItreeExtra/Secure/SecureEqEuttTrans.v
@@ -1,0 +1,154 @@
+From ITree Require Import
+     Axioms
+     ITree
+     ITreeFacts.
+
+From ITree.Extra Require Import
+     Secure.SecureEqHalt
+     Secure.SecureEqEuttHalt
+.
+
+From Paco Require Import paco.
+
+Import Monads.
+Import MonadNotation.
+Local Open Scope monad_scope.
+
+
+Lemma eses_aux3:
+  forall (E : Type -> Type) (R3 R1 : Type) (Label : Preorder)
+    (priv : forall A : Type, E A -> L) (l : L) (R2 : Type) (RR1 : R1 -> R2 -> Prop)
+    (RR2 : R2 -> R3 -> Prop) (r : itree E R1 -> itree E R3 -> Prop)
+    (m1 : itree E R2) (m2 : itree E R3),
+    paco2 (eqit_ RR2 true true id) bot2 m1 m2 ->
+    forall r0 : R1,
+      secure_eqitF Label priv RR1 true true l id
+                   (upaco2 (secure_eqit_ Label priv RR1 true true l id) bot2) (RetF r0)
+                   (observe m1) ->
+      secure_eqitF Label priv (rcompose RR1 RR2) true true l id
+                   (upaco2 (secure_eqit_ Label priv (rcompose RR1 RR2) true true l id) r)
+                   (RetF r0) (observe m2).
+Proof.
+  intros E R3 R1 Label priv l R2 RR1 RR2 r m1 m2 REL r0 Hsec.
+  remember (RetF r0) as x.
+  punfold REL. red in REL. hinduction Hsec before r; intros; inv Heqx; eauto.
+  - remember (RetF r2) as y. hinduction REL before r; intros; inv Heqy; eauto with itree.
+  - eapply IHHsec; eauto. pstep_reverse. setoid_rewrite <- tau_eutt at 1. pfold. auto.
+  - remember (VisF e k2) as y.
+    hinduction REL before r; intros; inv Heqy; ddestruction; subst; eauto with itree.
+    pclearbot. unpriv_ind. eapply H0; eauto. pstep_reverse.
+Qed.
+
+
+Lemma eses_aux4:
+  forall (E : Type -> Type) (R3 R1 : Type) (Label : Preorder)
+    (priv : forall A : Type, E A -> L) (l : L) (R2 : Type) (RR1 : R1 -> R2 -> Prop)
+    (RR2 : R2 -> R3 -> Prop) (r : itree E R1 -> itree E R3 -> Prop)
+    (m1 : itree E R2) (m2 : itree E R3),
+    (forall (t1 : itree E R1) (t2 : itree E R2) (t3 : itree E R3),
+        eqit_secure Label priv RR1 true true l t1 t2 -> eutt RR2 t2 t3 -> r t1 t3) ->
+    paco2 (eqit_ RR2 true true id) bot2 m1 m2 ->
+    forall (X : Type) (e : E X) (k : X -> itree E R1),
+      secure_eqitF Label priv RR1 true true l id
+                   (upaco2 (secure_eqit_ Label priv RR1 true true l id) bot2) (VisF e k)
+                   (observe m1) ->
+      leq (priv X e) l ->
+      secure_eqitF Label priv (rcompose RR1 RR2) true true l id
+                   (upaco2 (secure_eqit_ Label priv (rcompose RR1 RR2) true true l id) r)
+                   (VisF e k) (observe m2).
+Proof.
+  intros E R3 R1 Label priv l R2 RR1 RR2 r m1 m2 CIH REL X e k Hsec SECCHECK.
+  punfold REL. red in REL. remember (VisF e k) as y.
+  hinduction Hsec before r; intros; inv Heqy; ddestruction; subst; try contradiction.
+  - eapply IHHsec; eauto. pstep_reverse. rewrite <- tau_eutt at 1. pfold. auto.
+  - pclearbot. inv REL; ddestruction; subst.
+    + constructor; auto. right. pclearbot. eapply CIH; eauto with itree.
+      apply H.
+    + constructor; auto. remember (VisF e0 k2) as y.
+      hinduction REL0 before r; intros; inv Heqy; ddestruction; subst; try contradiction.
+      * constructor; auto. right. pclearbot. eapply CIH; eauto with itree. apply H.
+      * constructor; auto. eapply IHREL0; eauto.
+  - rewrite H2. remember (VisF e k2) as y.
+    hinduction REL before r; intros; inv Heqy; ddestruction; subst; try contradiction.
+    + rewrite itree_eta' at 1. unpriv_ind. rewrite <- H2. eapply H0; eauto.
+      pclearbot.
+      pstep_reverse.
+    + constructor; auto. eapply IHREL; eauto.
+Qed.
+
+(*This lemma lets us lift compiler correctness results to compiler security preservation results*)
+Lemma eutt_secure_eqit_secure : forall E Label priv l R1 R2 R3 (RR1 : R1 -> R2 -> Prop) (RR2 : R2 -> R3 -> Prop)
+  (t1 : itree E R1) (t2 : itree E R2) (t3 : itree E R3),
+    eqit_secure Label priv RR1 true true l t1 t2 -> eutt RR2 t2 t3 ->
+    eqit_secure Label priv (rcompose RR1 RR2) true true l t1 t3.
+Proof.
+  intros E Label priv l R1 R2 R3 RR1 RR2. pcofix CIH. intros t1 t2 t3 Hsec Heutt.
+  punfold Heutt. red in Heutt. punfold Hsec. red in Hsec.
+  pfold. red. hinduction Heutt before r; intros; subst; auto with itree.
+  - remember (RetF r2) as x. remember (RetF r1)  as y. hinduction Hsec before r; intros; try inv Heqx; try inv Heqy; subst; auto with itree.
+    + constructor; eauto with itree.
+    + constructor; auto. eapply IHHsec; eauto.
+    + rewrite itree_eta'. unpriv_ind. eapply H0; eauto.
+  - genobs_clear t1 ot1.
+    assert (Ht1 : (exists m3, ot1 = TauF m3) \/ (forall m3, ot1 <> TauF m3) ).
+    { destruct ot1; eauto; right; repeat intro; discriminate. }
+    (* because of the extra inductive cases this is not enough *)
+    destruct Ht1 as [ [m3 Hm3] | Ht1 ].
+    + subst. pclearbot. constructor. right. eapply CIH; eauto.
+      apply tau_eqit_secure. apply eqit_secure_sym. apply tau_eqit_secure.
+      apply eqit_secure_sym. pfold. auto.
+    + destruct ot1; try (exfalso; eapply Ht1; eauto; fail).
+      * pclearbot. rewrite itree_eta'. rewrite itree_eta' in Hsec.
+        eapply eses_aux3; eauto. pfold. constructor.
+        left. auto.
+      * assert (leq (priv _ e) l \/ ~ leq (priv _ e) l).
+        { apply classic. }
+        destruct H as [SECCHECK | SECCHECK]; destruct ( classic_empty X  ).
+        ++ pclearbot. rewrite itree_eta'. rewrite itree_eta' in Hsec.
+           eapply eses_aux4; eauto. do 2 rewrite tau_eutt. auto.
+        ++ pclearbot. rewrite itree_eta'.
+           rewrite itree_eta' in Hsec. eapply eses_aux4; eauto.
+           do 2 rewrite tau_eutt. auto.
+        ++ unpriv_halt. pclearbot. right. eapply CIH; eauto.
+           apply eqit_secure_sym. apply tau_eqit_secure. apply eqit_secure_sym.
+           pfold. auto.
+        ++ pclearbot.
+           unpriv_co. pclearbot. right. eapply CIH; try apply REL.
+           apply eqit_secure_sym. apply tau_eqit_secure.
+           apply eqit_secure_sym.
+           eapply unpriv_e_eqit_secure; eauto.
+           pfold. auto.
+  - pclearbot. destruct (classic (leq (priv _ e) l ) ).
+    + genobs_clear t1 ot1.
+      remember (VisF e k1) as y.
+      hinduction Hsec before r; intros; try inv Heqy; ddestruction; subst; try contradiction;
+      eauto with itree.
+      * constructor; auto. right. pclearbot. eapply CIH; eauto with itree. apply H.
+      * rewrite itree_eta'. unpriv_ind. eapply H0; eauto.
+    + remember (VisF e k1) as y.
+      hinduction Hsec before r; intros; inv Heqy; ddestruction; subst; try contradiction.
+      * eauto with itree.
+      * pclearbot. unpriv_co. right. eapply CIH; eauto with itree. apply H.
+      * pclearbot. unpriv_co. right. eapply CIH; eauto with itree. apply H.
+      * rewrite itree_eta'. unpriv_ind. eapply H0; eauto.
+      * destruct (observe t0).
+        -- rewrite itree_eta' at 1. unpriv_ind.
+           specialize (H a).
+           eapply eses_aux3; eauto.
+        -- unpriv_co. right. eapply CIH; eauto with itree. apply tau_eqit_secure.
+           pfold. apply H.
+        -- destruct (classic (leq (priv _ e) l ) ).
+           ++ rewrite itree_eta' at 1. unpriv_ind.
+              eapply eses_aux4; eauto.
+           ++ destruct (classic_empty X).
+              ** unpriv_halt. right. eapply CIH; eauto with itree. pfold. apply H.
+              ** unpriv_co. right. eapply CIH; eauto with itree.
+                 eapply unpriv_e_eqit_secure; eauto. pfold. apply H.
+      * pclearbot. unpriv_halt. right. eapply CIH; eauto. pfold.
+        constructor; intros; auto with itree.
+      * pclearbot. unpriv_halt. right. eapply CIH; eauto with itree. apply H.
+      * pclearbot. unpriv_halt. right. eapply CIH; eauto with itree. apply H.
+        pfold. constructor; auto with itree.
+  - eapply IHHeutt; eauto. pstep_reverse. apply eqit_secure_sym.
+    apply tau_eqit_secure. apply eqit_secure_sym. pfold. auto.
+Qed.
